<?xml version="1.0" encoding="utf-16"?>
<!DOCTYPE rdf:RDF [
	<!ENTITY rdf 'http://www.w3.org/1999/02/22-rdf-syntax-ns#'>
	<!ENTITY rdfs 'http://www.w3.org/2000/01/rdf-schema#'>
	<!ENTITY xsd 'http://www.w3.org/2001/XMLSchema#'>
	<!ENTITY owl 'http://www.w3.org/2002/07/owl#'>
	<!ENTITY xml 'http://www.w3.org/XML/1998/namespace'>
]>
<rdf:RDF xml:base="http://geographicknowledge.de/vocab/CoreConceptData.rdf" xmlns:rdfs="http://www.w3.org/2000/01/rdf-schema#" xmlns:xsd="http://www.w3.org/2001/XMLSchema#" xmlns="http://geographicknowledge.de/vocab/CoreConceptData.rdf#" xmlns:owl="http://www.w3.org/2002/07/owl#" xmlns:xml="http://www.w3.org/XML/1998/namespace" xmlns:rdf="http://www.w3.org/1999/02/22-rdf-syntax-ns#">
  <owl:Class rdf:about="http://geographicknowledge.de/vocab/AnalysisData.rdf#Attribute">
    <owl:equivalentClass rdf:resource="http://geographicknowledge.de/vocab/CoreConceptData.rdf#Attribute" />
  </owl:Class>
  <owl:Class rdf:about="http://geographicknowledge.de/vocab/AnalysisData.rdf#Quality" />
  <owl:Class rdf:about="http://geographicknowledge.de/vocab/AnalysisData.rdf#Spatial" />
  <owl:Class rdf:about="http://geographicknowledge.de/vocab/AnalysisData.rdf#SpatialData" />
  <owl:Class rdf:about="http://geographicknowledge.de/vocab/AnalysisData.rdf#SpatialDataSet" />
  <owl:ObjectProperty rdf:about="http://geographicknowledge.de/vocab/AnalysisData.rdf#hasElement" />
  <rdf:Description rdf:about="http://geographicknowledge.de/vocab/AnalysisData.rdf#measureConnect" rdfs:comment="ofDataSet o hasElement o hasMeasure o valueOf" />
  <owl:ObjectProperty rdf:about="http://geographicknowledge.de/vocab/AnalysisData.rdf#ofDataSet" />
  <rdf:Description rdf:about="http://geographicknowledge.de/vocab/AnalysisData.rdf#supportConnect" rdfs:comment="ofDataSet o hasElement o hasSupport o valueOf" />
  <owl:Ontology rdf:about="http://geographicknowledge.de/vocab/CoreConceptData.rdf">
    <rdfs:comment xml:lang="en">This ontology pattern describes geodata types representing core concepts of spatial information (Kuhn 2012) we well as further semantic attribute distinctions relevant for geocomputation and geo-analysis. The ontology was introduced in: Scheider et la. (2020): Ontology of core concept data types for answering geo-analytical questions. Journal of Spatial Information Science 20 (2020): 167-201. https://josis.org/index.php/josis/article/view/125 </rdfs:comment>
    <rdfs:seeAlso rdf:resource="http://spatial.ucsb.edu/core-concepts-of-spatial-information/" />
  </owl:Ontology>
  <owl:Class rdf:about="http://geographicknowledge.de/vocab/CoreConceptData.rdf#AmountDS">
    <rdfs:comment xml:lang="en">Dataset of amounts of objects</rdfs:comment>
    <rdfs:subClassOf rdf:resource="http://geographicknowledge.de/vocab/CoreConceptData.rdf#CoreConceptDataSet" />
  </owl:Class>
  <owl:Class rdf:about="http://geographicknowledge.de/vocab/CoreConceptData.rdf#AmountQ">
    <rdfs:comment xml:lang="en">An attribute that represents a (quantified) amount, which is a quantity defined by an arbitrary part of space. This can be either an amount of objects or an amount of some field.</rdfs:comment>
    <rdfs:subClassOf rdf:resource="http://geographicknowledge.de/vocab/CoreConceptData.rdf#CoreConceptQ" />
    <owl:equivalentClass>
      <owl:Restriction>
        <owl:onProperty rdf:resource="http://geographicknowledge.de/vocab/AnalysisData.rdf#ofDataSet" />
        <owl:someValuesFrom rdf:resource="http://geographicknowledge.de/vocab/CoreConceptData.rdf#AmountDS" />
      </owl:Restriction>
    </owl:equivalentClass>
  </owl:Class>
  <owl:Class rdf:about="http://geographicknowledge.de/vocab/CoreConceptData.rdf#AmountRasterDS">
    <rdfs:comment xml:lang="en">A raster data set where each cell represents an amount of objects</rdfs:comment>
    <rdfs:subClassOf rdf:resource="http://geographicknowledge.de/vocab/CoreConceptData.rdf#AmountDS" />
    <owl:equivalentClass>
      <owl:Class>
        <owl:intersectionOf rdf:nodeID="autos260" />
      </owl:Class>
    </owl:equivalentClass>
  </owl:Class>
  <owl:Class rdf:about="http://geographicknowledge.de/vocab/CoreConceptData.rdf#AmountVectorDS">
    <rdfs:comment xml:lang="en">A dataset where each geometry denotes an amount of objects</rdfs:comment>
    <rdfs:subClassOf rdf:resource="http://geographicknowledge.de/vocab/CoreConceptData.rdf#AmountDS" />
    <owl:equivalentClass>
      <owl:Class>
        <owl:intersectionOf rdf:nodeID="autos263" />
      </owl:Class>
    </owl:equivalentClass>
  </owl:Class>
  <owl:Class rdf:about="http://geographicknowledge.de/vocab/CoreConceptData.rdf#Attribute">
    <rdfs:comment xml:lang="en">Attributes of a tabular dataset. Each attribute corresponds to a column in the table.</rdfs:comment>
  </owl:Class>
  <owl:Class rdf:about="http://geographicknowledge.de/vocab/CoreConceptData.rdf#BooleanA">
    <rdfs:comment xml:lang="en">Boolean attributes are spatial attributes within the range of True/False. They are special types of (bi)nominal attributes</rdfs:comment>
    <rdfs:subClassOf rdf:resource="http://geographicknowledge.de/vocab/CoreConceptData.rdf#NominalA" />
  </owl:Class>
  <owl:Class rdf:about="http://geographicknowledge.de/vocab/CoreConceptData.rdf#BoundedPhen">
    <rdfs:comment xml:lang="en">This is a spatial attribute which denotes a bounded phenomenon. Can be either a object vector or an existence raster</rdfs:comment>
    <rdfs:subClassOf rdf:resource="http://geographicknowledge.de/vocab/CoreConceptData.rdf#Attribute" />
    <owl:equivalentClass>
      <owl:Class>
        <owl:unionOf rdf:nodeID="autos266" />
      </owl:Class>
    </owl:equivalentClass>
  </owl:Class>
  <owl:Class rdf:about="http://geographicknowledge.de/vocab/CoreConceptData.rdf#Contour">
    <rdfs:comment xml:lang="en">Contour layers are coverages that denote intervals of the reprepresented continuous field. For example, temperature intervals, represented as regions bounded by isolines of a temperature field.</rdfs:comment>
    <rdfs:subClassOf rdf:resource="http://geographicknowledge.de/vocab/CoreConceptData.rdf#Coverage" />
    <rdfs:subClassOf rdf:resource="http://geographicknowledge.de/vocab/CoreConceptData.rdf#OrdinalA" />
  </owl:Class>
  <owl:Class rdf:about="http://geographicknowledge.de/vocab/CoreConceptData.rdf#ContourDS">
    <rdfs:comment xml:lang="en">A dataset representing a field using contours, which denote the boundaries of value intervals. For example, a terrain contour map.</rdfs:comment>
    <rdfs:subClassOf rdf:resource="http://geographicknowledge.de/vocab/CoreConceptData.rdf#CoverageDS" />
  </owl:Class>
  <owl:Class rdf:about="http://geographicknowledge.de/vocab/CoreConceptData.rdf#CoreConceptDataSet">
    <rdfs:comment xml:lang="en">A data set which represents a core concept of spatial information. The attributes of this dataset are assumed to be of corresponding types.</rdfs:comment>
    <rdfs:subClassOf rdf:resource="http://geographicknowledge.de/vocab/AnalysisData.rdf#SpatialDataSet" />
  </owl:Class>
  <owl:Class rdf:about="http://geographicknowledge.de/vocab/CoreConceptData.rdf#CoreConceptQ">
    <rdfs:comment xml:lang="en">Superclass of all core concept qualities.</rdfs:comment>
    <rdfs:subClassOf rdf:resource="http://geographicknowledge.de/vocab/CoreConceptData.rdf#Attribute" />
  </owl:Class>
  <owl:Class rdf:about="http://geographicknowledge.de/vocab/CoreConceptData.rdf#CountA">
    <rdfs:comment xml:lang="en">An attribute that denotes counts of discrete entities (compare Chrisman 1998)</rdfs:comment>
    <rdfs:subClassOf rdf:resource="http://geographicknowledge.de/vocab/CoreConceptData.rdf#RatioA" />
  </owl:Class>
  <owl:Class rdf:about="http://geographicknowledge.de/vocab/CoreConceptData.rdf#Coverage">
    <rdfs:comment xml:lang="en">Coverages are tessellated layers that represent a continuous field. For example, landuse polygons.</rdfs:comment>
    <rdfs:subClassOf rdf:resource="http://geographicknowledge.de/vocab/CoreConceptData.rdf#FieldQ" />
    <rdfs:subClassOf rdf:resource="http://geographicknowledge.de/vocab/CoreConceptData.rdf#TessellationA" />
    <owl:equivalentClass>
      <owl:Class>
        <owl:intersectionOf rdf:nodeID="autos270" />
      </owl:Class>
    </owl:equivalentClass>
  </owl:Class>
  <owl:Class rdf:about="http://geographicknowledge.de/vocab/CoreConceptData.rdf#CoverageDS">
    <rdfs:comment xml:lang="en">A dataset representing a field using (possibly irregular) patches of homogeneous values. For example, a landuse map or a soil map.</rdfs:comment>
    <rdfs:subClassOf rdf:resource="http://geographicknowledge.de/vocab/CoreConceptData.rdf#FieldDS" />
    <owl:equivalentClass>
      <owl:Class>
        <owl:intersectionOf rdf:nodeID="autos274" />
      </owl:Class>
    </owl:equivalentClass>
  </owl:Class>
  <owl:Class rdf:about="http://geographicknowledge.de/vocab/CoreConceptData.rdf#CyclicA">
    <rdfs:comment xml:lang="en">An attribute that denotes a cyclical measure, like an angle. Note that cyclical measures don't have a natural ordering and thus are not ordinal scaled. (compare Chrisman 1998)</rdfs:comment>
    <rdfs:subClassOf rdf:resource="http://geographicknowledge.de/vocab/CoreConceptData.rdf#NominalA" />
  </owl:Class>
  <owl:Class rdf:about="http://geographicknowledge.de/vocab/CoreConceptData.rdf#EventDS">
    <rdfs:comment xml:lang="en">A spatial dataset representing events</rdfs:comment>
    <rdfs:subClassOf rdf:resource="http://geographicknowledge.de/vocab/CoreConceptData.rdf#CoreConceptDataSet" />
  </owl:Class>
  <owl:Class rdf:about="http://geographicknowledge.de/vocab/CoreConceptData.rdf#EventQ">
    <rdfs:comment xml:lang="en">This attribute represents a quality of an event (core concept). For example, the duration.</rdfs:comment>
    <rdfs:subClassOf rdf:resource="http://geographicknowledge.de/vocab/CoreConceptData.rdf#CoreConceptQ" />
    <owl:equivalentClass>
      <owl:Restriction>
        <owl:onProperty rdf:resource="http://geographicknowledge.de/vocab/AnalysisData.rdf#ofDataSet" />
        <owl:someValuesFrom rdf:resource="http://geographicknowledge.de/vocab/CoreConceptData.rdf#EventDS" />
      </owl:Restriction>
    </owl:equivalentClass>
  </owl:Class>
  <owl:Class rdf:about="http://geographicknowledge.de/vocab/CoreConceptData.rdf#EventVector">
    <rdfs:comment xml:lang="en">Events represented in terms of an attribute of a vector data set. For example, the magnitude of earthquakes represented as an attribute of a point data set.</rdfs:comment>
    <rdfs:subClassOf rdf:resource="http://geographicknowledge.de/vocab/CoreConceptData.rdf#EventQ" />
    <rdfs:subClassOf rdf:resource="http://geographicknowledge.de/vocab/CoreConceptData.rdf#VectorA" />
    <owl:equivalentClass>
      <owl:Class>
        <owl:intersectionOf rdf:nodeID="autos278" />
      </owl:Class>
    </owl:equivalentClass>
  </owl:Class>
  <owl:Class rdf:about="http://geographicknowledge.de/vocab/CoreConceptData.rdf#ExistenceRaster">
    <rdfs:comment xml:lang="en">Existence rasters are rasters representing boolean fields (fields denoting whether something is present at a cell location or not).</rdfs:comment>
    <rdfs:subClassOf rdf:resource="http://geographicknowledge.de/vocab/CoreConceptData.rdf#BooleanA" />
    <rdfs:subClassOf rdf:resource="http://geographicknowledge.de/vocab/CoreConceptData.rdf#BoundedPhen" />
    <rdfs:subClassOf rdf:resource="http://geographicknowledge.de/vocab/CoreConceptData.rdf#FieldRaster" />
    <owl:equivalentClass>
      <owl:Class>
        <owl:intersectionOf rdf:nodeID="autos282" />
      </owl:Class>
    </owl:equivalentClass>
  </owl:Class>
  <owl:Class rdf:about="http://geographicknowledge.de/vocab/CoreConceptData.rdf#ExistenceVector">
    <rdfs:comment xml:lang="en">A vector layer attribute that satisfies a boolean expression and thus denotes the 'existence' of some attribute encoded phenomenon across space. Example is a layer of polygons of ''forest'' landuse or a layer of "parks".</rdfs:comment>
    <rdfs:subClassOf rdf:resource="http://geographicknowledge.de/vocab/CoreConceptData.rdf#BooleanA" />
    <rdfs:subClassOf rdf:resource="http://geographicknowledge.de/vocab/CoreConceptData.rdf#BoundedPhen" />
    <rdfs:subClassOf rdf:resource="http://geographicknowledge.de/vocab/CoreConceptData.rdf#FieldVector" />
    <rdfs:subClassOf rdf:resource="http://geographicknowledge.de/vocab/CoreConceptData.rdf#VectorA" />
    <owl:equivalentClass>
      <owl:Class>
        <owl:intersectionOf rdf:nodeID="autos285" />
      </owl:Class>
    </owl:equivalentClass>
  </owl:Class>
  <owl:Class rdf:about="http://geographicknowledge.de/vocab/CoreConceptData.rdf#ExtLattice">
    <rdfs:comment xml:lang="en">This type of lattice has an extensive attribute. For example, a spatial dataset about the population number of municipalities</rdfs:comment>
    <rdfs:subClassOf rdf:resource="http://geographicknowledge.de/vocab/CoreConceptData.rdf#Lattice" />
    <rdfs:subClassOf rdf:resource="http://geographicknowledge.de/vocab/ExtensiveMeasures.rdf#ERA" />
    <owl:equivalentClass>
      <owl:Class>
        <owl:intersectionOf rdf:nodeID="autos288" />
      </owl:Class>
    </owl:equivalentClass>
  </owl:Class>
  <owl:Class rdf:about="http://geographicknowledge.de/vocab/CoreConceptData.rdf#FieldDS">
    <rdfs:comment xml:lang="en">A spatial dataset representing a field</rdfs:comment>
    <rdfs:subClassOf rdf:resource="http://geographicknowledge.de/vocab/CoreConceptData.rdf#CoreConceptDataSet" />
  </owl:Class>
  <owl:Class rdf:about="http://geographicknowledge.de/vocab/CoreConceptData.rdf#FieldQ">
    <rdfs:comment xml:lang="en">An attribute which represents the quality of a field (core concept). This implies that the spatial data items in this data set are self-similar (their parts have the same attribute)</rdfs:comment>
    <rdfs:subClassOf rdf:resource="http://geographicknowledge.de/vocab/CoreConceptData.rdf#CoreConceptQ" />
    <owl:equivalentClass>
      <owl:Restriction>
        <owl:onProperty rdf:resource="http://geographicknowledge.de/vocab/AnalysisData.rdf#ofDataSet" />
        <owl:someValuesFrom rdf:resource="http://geographicknowledge.de/vocab/CoreConceptData.rdf#FieldDS" />
      </owl:Restriction>
    </owl:equivalentClass>
  </owl:Class>
  <owl:Class rdf:about="http://geographicknowledge.de/vocab/CoreConceptData.rdf#FieldRaster">
    <rdfs:comment xml:lang="en">Field rasters are raster representations of continuous fields. For example, raster layers representing a terrain height (DTM).</rdfs:comment>
    <rdfs:subClassOf rdf:resource="http://geographicknowledge.de/vocab/CoreConceptData.rdf#FieldQ" />
    <rdfs:subClassOf rdf:resource="http://geographicknowledge.de/vocab/CoreConceptData.rdf#RasterA" />
    <owl:equivalentClass>
      <owl:Class>
        <owl:intersectionOf rdf:nodeID="autos292" />
      </owl:Class>
    </owl:equivalentClass>
  </owl:Class>
  <owl:Class rdf:about="http://geographicknowledge.de/vocab/CoreConceptData.rdf#FieldRasterDS">
    <rdfs:comment xml:lang="en">A dataset representing a field by homogeneous values using raster cells</rdfs:comment>
    <rdfs:subClassOf rdf:resource="http://geographicknowledge.de/vocab/CoreConceptData.rdf#FieldDS" />
    <owl:equivalentClass>
      <owl:Class>
        <owl:intersectionOf rdf:nodeID="autos296" />
      </owl:Class>
    </owl:equivalentClass>
  </owl:Class>
  <owl:Class rdf:about="http://geographicknowledge.de/vocab/CoreConceptData.rdf#FieldVector">
    <rdfs:comment xml:lang="en">A vector representation of a field. Can be a point or line measure, or a coverage, or a Patch</rdfs:comment>
    <rdfs:subClassOf rdf:resource="http://geographicknowledge.de/vocab/CoreConceptData.rdf#FieldQ" />
    <rdfs:subClassOf rdf:resource="http://geographicknowledge.de/vocab/CoreConceptData.rdf#VectorA" />
    <owl:equivalentClass>
      <owl:Class>
        <owl:intersectionOf rdf:nodeID="autos299" />
      </owl:Class>
    </owl:equivalentClass>
  </owl:Class>
  <owl:Class rdf:about="http://geographicknowledge.de/vocab/CoreConceptData.rdf#IntervalA">
    <rdfs:comment xml:lang="en">An interval scaled attribute</rdfs:comment>
    <rdfs:subClassOf rdf:resource="http://geographicknowledge.de/vocab/CoreConceptData.rdf#OrdinalA" />
  </owl:Class>
  <owl:Class rdf:about="http://geographicknowledge.de/vocab/CoreConceptData.rdf#Lattice">
    <rdfs:comment xml:lang="en">A lattice is a spatial tessellation that represents objects and their qualities. For example, a set of municipalities with average income.</rdfs:comment>
    <rdfs:subClassOf rdf:resource="http://geographicknowledge.de/vocab/CoreConceptData.rdf#ObjectQ" />
    <rdfs:subClassOf rdf:resource="http://geographicknowledge.de/vocab/CoreConceptData.rdf#TessellationA" />
    <owl:equivalentClass>
      <owl:Class>
        <owl:intersectionOf rdf:nodeID="autos303" />
      </owl:Class>
    </owl:equivalentClass>
  </owl:Class>
  <owl:Class rdf:about="http://geographicknowledge.de/vocab/CoreConceptData.rdf#LatticeDS">
    <rdfs:comment xml:lang="en">A dataset of objects which tesselate space and contain statistical summaries. For example, the municipalities of the Netherlands</rdfs:comment>
    <rdfs:subClassOf rdf:resource="http://geographicknowledge.de/vocab/CoreConceptData.rdf#ObjectDS" />
    <owl:equivalentClass>
      <owl:Class>
        <owl:intersectionOf rdf:nodeID="autos307" />
      </owl:Class>
    </owl:equivalentClass>
  </owl:Class>
  <owl:Class rdf:about="http://geographicknowledge.de/vocab/CoreConceptData.rdf#LayerA">
    <rdfs:comment xml:lang="en">Superclass of of attribute types that characterize a geometric layer property</rdfs:comment>
    <rdfs:subClassOf rdf:resource="http://geographicknowledge.de/vocab/CoreConceptData.rdf#Attribute" />
  </owl:Class>
  <owl:Class rdf:about="http://geographicknowledge.de/vocab/CoreConceptData.rdf#Line">
    <rdfs:comment xml:lang="en">A generalized notion of a line in 2D and 3D</rdfs:comment>
    <rdfs:subClassOf rdf:resource="http://geographicknowledge.de/vocab/AnalysisData.rdf#Spatial" />
  </owl:Class>
  <owl:Class rdf:about="http://geographicknowledge.de/vocab/CoreConceptData.rdf#LineA">
    <rdfs:comment xml:lang="en">Attribute of some Line data set</rdfs:comment>
    <rdfs:subClassOf rdf:resource="http://geographicknowledge.de/vocab/CoreConceptData.rdf#VectorA" />
    <owl:equivalentClass>
      <owl:Class>
        <owl:intersectionOf rdf:nodeID="autos310" />
      </owl:Class>
    </owl:equivalentClass>
  </owl:Class>
  <owl:Class rdf:about="http://geographicknowledge.de/vocab/CoreConceptData.rdf#LineDS">
    <owl:disjointWith rdf:resource="http://geographicknowledge.de/vocab/CoreConceptData.rdf#PointDS" />
    <owl:disjointWith rdf:resource="http://geographicknowledge.de/vocab/CoreConceptData.rdf#RegionDS" />
    <owl:equivalentClass>
      <owl:Class>
        <owl:intersectionOf rdf:nodeID="autos314" />
      </owl:Class>
    </owl:equivalentClass>
  </owl:Class>
  <owl:Class rdf:about="http://geographicknowledge.de/vocab/CoreConceptData.rdf#LineData">
    <owl:equivalentClass>
      <owl:Class>
        <owl:intersectionOf rdf:nodeID="autos318" />
      </owl:Class>
    </owl:equivalentClass>
  </owl:Class>
  <owl:Class rdf:about="http://geographicknowledge.de/vocab/CoreConceptData.rdf#LineMeasures">
    <rdfs:comment xml:lang="en">Linear representations of fields. Examples are isoline maps</rdfs:comment>
    <rdfs:subClassOf rdf:resource="http://geographicknowledge.de/vocab/CoreConceptData.rdf#FieldQ" />
    <rdfs:subClassOf rdf:resource="http://geographicknowledge.de/vocab/CoreConceptData.rdf#LineA" />
    <owl:equivalentClass>
      <owl:Class>
        <owl:intersectionOf rdf:nodeID="autos322" />
      </owl:Class>
    </owl:equivalentClass>
  </owl:Class>
  <owl:Class rdf:about="http://geographicknowledge.de/vocab/CoreConceptData.rdf#LineMeasuresDS">
    <rdfs:comment xml:lang="en">A representation of a field as a line of homogeneous values</rdfs:comment>
    <rdfs:subClassOf rdf:resource="http://geographicknowledge.de/vocab/CoreConceptData.rdf#FieldDS" />
    <owl:equivalentClass>
      <owl:Class>
        <owl:intersectionOf rdf:nodeID="autos326" />
      </owl:Class>
    </owl:equivalentClass>
  </owl:Class>
  <owl:Class rdf:about="http://geographicknowledge.de/vocab/CoreConceptData.rdf#MatrixDS">
    <rdfs:comment xml:lang="en">A network relation where the complete cross-product of an object domain forms the key. Examples would be origin-destination matrices.</rdfs:comment>
    <rdfs:subClassOf rdf:resource="http://geographicknowledge.de/vocab/CoreConceptData.rdf#RelationalDS" />
  </owl:Class>
  <owl:Class rdf:about="http://geographicknowledge.de/vocab/CoreConceptData.rdf#MatrixQ">
    <rdfs:comment xml:lang="en">an attribute of a matrix. For example, distance in an origin-destination matrix.</rdfs:comment>
    <rdfs:subClassOf rdf:resource="http://geographicknowledge.de/vocab/CoreConceptData.rdf#RelationalQ" />
    <owl:equivalentClass>
      <owl:Restriction>
        <owl:onProperty rdf:resource="http://geographicknowledge.de/vocab/AnalysisData.rdf#ofDataSet" />
        <owl:someValuesFrom rdf:resource="http://geographicknowledge.de/vocab/CoreConceptData.rdf#MatrixDS" />
      </owl:Restriction>
    </owl:equivalentClass>
  </owl:Class>
  <owl:Class rdf:about="http://geographicknowledge.de/vocab/CoreConceptData.rdf#NetworkDS">
    <rdfs:comment xml:lang="en">A spatial dataset representing a spatial network. Note thate a network in the sense of a core concept is a quantified relation between objects. For example, the traffic flow between municipalities or between two intersections. Streets themselves can also be seen as objects if they do not encode such relations</rdfs:comment>
    <rdfs:subClassOf rdf:resource="http://geographicknowledge.de/vocab/CoreConceptData.rdf#RelationalDS" />
  </owl:Class>
  <owl:Class rdf:about="http://geographicknowledge.de/vocab/CoreConceptData.rdf#NetworkQ">
    <rdfs:comment xml:lang="en">This attribute represents the quality of a network edge. Note that spatial networks (as core concepts) are regarded as quantified relations between objects. So O-IRA-O would be an intensive quality measured between two objects, such as their distance from each other.</rdfs:comment>
    <rdfs:subClassOf rdf:resource="http://geographicknowledge.de/vocab/CoreConceptData.rdf#RelationalQ" />
    <owl:equivalentClass>
      <owl:Restriction>
        <owl:onProperty rdf:resource="http://geographicknowledge.de/vocab/AnalysisData.rdf#ofDataSet" />
        <owl:someValuesFrom rdf:resource="http://geographicknowledge.de/vocab/CoreConceptData.rdf#NetworkDS" />
      </owl:Restriction>
    </owl:equivalentClass>
  </owl:Class>
  <owl:Class rdf:about="http://geographicknowledge.de/vocab/CoreConceptData.rdf#NoDataExistenceRaster">
    <rdfs:comment xml:lang="en">A raster dataset where  NoData is interpreted as boolean "false".</rdfs:comment>
    <rdfs:subClassOf rdf:resource="http://geographicknowledge.de/vocab/CoreConceptData.rdf#ExistenceRaster" />
  </owl:Class>
  <owl:Class rdf:about="http://geographicknowledge.de/vocab/CoreConceptData.rdf#NominalA">
    <rdfs:comment xml:lang="en">A spatial attribute on nominal scale level</rdfs:comment>
    <rdfs:subClassOf rdf:resource="http://geographicknowledge.de/vocab/CoreConceptData.rdf#Attribute" />
  </owl:Class>
  <owl:Class rdf:about="http://geographicknowledge.de/vocab/CoreConceptData.rdf#ObjectDS">
    <rdfs:comment xml:lang="en">A spatial data set representing objects</rdfs:comment>
    <rdfs:subClassOf rdf:resource="http://geographicknowledge.de/vocab/CoreConceptData.rdf#CoreConceptDataSet" />
  </owl:Class>
  <owl:Class rdf:about="http://geographicknowledge.de/vocab/CoreConceptData.rdf#ObjectLine">
    <rdfs:comment xml:lang="en">An attribute of an object line dataset</rdfs:comment>
    <rdfs:subClassOf rdf:resource="http://geographicknowledge.de/vocab/CoreConceptData.rdf#LineA" />
    <rdfs:subClassOf rdf:resource="http://geographicknowledge.de/vocab/CoreConceptData.rdf#ObjectQ" />
    <owl:equivalentClass>
      <owl:Class>
        <owl:intersectionOf rdf:nodeID="autos331" />
      </owl:Class>
    </owl:equivalentClass>
  </owl:Class>
  <owl:Class rdf:about="http://geographicknowledge.de/vocab/CoreConceptData.rdf#ObjectPoint">
    <rdfs:comment xml:lang="en">An attribute of an object point dataset</rdfs:comment>
    <rdfs:subClassOf rdf:resource="http://geographicknowledge.de/vocab/CoreConceptData.rdf#ObjectQ" />
    <rdfs:subClassOf rdf:resource="http://geographicknowledge.de/vocab/CoreConceptData.rdf#PointA" />
    <owl:equivalentClass>
      <owl:Class>
        <owl:intersectionOf rdf:nodeID="autos335" />
      </owl:Class>
    </owl:equivalentClass>
  </owl:Class>
  <owl:Class rdf:about="http://geographicknowledge.de/vocab/CoreConceptData.rdf#ObjectQ">
    <rdfs:comment xml:lang="en">An attribute that represents the quality of an object (core concept)</rdfs:comment>
    <rdfs:subClassOf rdf:resource="http://geographicknowledge.de/vocab/CoreConceptData.rdf#CoreConceptQ" />
    <owl:equivalentClass>
      <owl:Restriction>
        <owl:onProperty rdf:resource="http://geographicknowledge.de/vocab/AnalysisData.rdf#ofDataSet" />
        <owl:someValuesFrom rdf:resource="http://geographicknowledge.de/vocab/CoreConceptData.rdf#ObjectDS" />
      </owl:Restriction>
    </owl:equivalentClass>
  </owl:Class>
  <owl:Class rdf:about="http://geographicknowledge.de/vocab/CoreConceptData.rdf#ObjectRegion">
    <rdfs:subClassOf rdf:resource="http://geographicknowledge.de/vocab/CoreConceptData.rdf#ObjectQ" />
    <rdfs:subClassOf rdf:resource="http://geographicknowledge.de/vocab/CoreConceptData.rdf#RegionA" />
    <owl:equivalentClass>
      <owl:Class>
        <owl:intersectionOf rdf:nodeID="autos340" />
      </owl:Class>
    </owl:equivalentClass>
  </owl:Class>
  <owl:Class rdf:about="http://geographicknowledge.de/vocab/CoreConceptData.rdf#ObjectVector">
    <rdfs:comment xml:lang="en">Object vectors are vector representation of a set of objecs and their quality. For example, a point layer denoting points of Interest (POI) or buildings in a city together with their quality, e.g. the building height.</rdfs:comment>
    <rdfs:subClassOf rdf:resource="http://geographicknowledge.de/vocab/CoreConceptData.rdf#BoundedPhen" />
    <rdfs:subClassOf rdf:resource="http://geographicknowledge.de/vocab/CoreConceptData.rdf#ObjectQ" />
    <rdfs:subClassOf rdf:resource="http://geographicknowledge.de/vocab/CoreConceptData.rdf#VectorA" />
    <owl:equivalentClass>
      <owl:Class>
        <owl:intersectionOf rdf:nodeID="autos344" />
      </owl:Class>
    </owl:equivalentClass>
  </owl:Class>
  <owl:Class rdf:about="http://geographicknowledge.de/vocab/CoreConceptData.rdf#OrdinalA">
    <rdfs:comment xml:lang="en">A spatial attribute on ordinal scale level</rdfs:comment>
    <rdfs:subClassOf rdf:resource="http://geographicknowledge.de/vocab/CoreConceptData.rdf#NominalA" />
  </owl:Class>
  <owl:Class rdf:about="http://geographicknowledge.de/vocab/CoreConceptData.rdf#Patch">
    <rdfs:comment xml:lang="en">An attribute of some dataset representing homogeneous patches of a field as regions.</rdfs:comment>
    <rdfs:subClassOf rdf:resource="http://geographicknowledge.de/vocab/CoreConceptData.rdf#FieldQ" />
    <rdfs:subClassOf rdf:resource="http://geographicknowledge.de/vocab/CoreConceptData.rdf#RegionA" />
    <owl:equivalentClass>
      <owl:Class>
        <owl:intersectionOf rdf:nodeID="autos348" />
      </owl:Class>
    </owl:equivalentClass>
  </owl:Class>
  <owl:Class rdf:about="http://geographicknowledge.de/vocab/CoreConceptData.rdf#PatchDS">
    <rdfs:comment xml:lang="en">A dataset which represents a field in terms patches of homogeneous values. Not necessarily tessellated</rdfs:comment>
    <rdfs:subClassOf rdf:resource="http://geographicknowledge.de/vocab/CoreConceptData.rdf#FieldDS" />
    <owl:equivalentClass>
      <owl:Class>
        <owl:intersectionOf rdf:nodeID="autos352" />
      </owl:Class>
    </owl:equivalentClass>
  </owl:Class>
  <owl:Class rdf:about="http://geographicknowledge.de/vocab/CoreConceptData.rdf#PlainIntervalA">
    <rdfs:comment xml:lang="en">An interval attribute that is plain/proper</rdfs:comment>
    <rdfs:subClassOf rdf:resource="http://geographicknowledge.de/vocab/CoreConceptData.rdf#IntervalA" />
    <owl:equivalentClass>
      <owl:Class>
        <owl:intersectionOf rdf:nodeID="autos355" />
      </owl:Class>
    </owl:equivalentClass>
  </owl:Class>
  <owl:Class rdf:about="http://geographicknowledge.de/vocab/CoreConceptData.rdf#PlainNominalA">
    <rdfs:comment xml:lang="en">A nominal attribute that is plain/proper (not ordinal or boolean)</rdfs:comment>
    <rdfs:subClassOf rdf:resource="http://geographicknowledge.de/vocab/CoreConceptData.rdf#NominalA" />
    <owl:equivalentClass>
      <owl:Class>
        <owl:intersectionOf rdf:nodeID="autos359" />
      </owl:Class>
    </owl:equivalentClass>
  </owl:Class>
  <owl:Class rdf:about="http://geographicknowledge.de/vocab/CoreConceptData.rdf#PlainOrdinalA">
    <rdfs:comment xml:lang="en">An ordinal attribute that is plain/proper (not interval)</rdfs:comment>
    <rdfs:subClassOf rdf:resource="http://geographicknowledge.de/vocab/CoreConceptData.rdf#OrdinalA" />
    <owl:equivalentClass>
      <owl:Class>
        <owl:intersectionOf rdf:nodeID="autos363" />
      </owl:Class>
    </owl:equivalentClass>
  </owl:Class>
  <owl:Class rdf:about="http://geographicknowledge.de/vocab/CoreConceptData.rdf#PlainRatioA">
    <rdfs:comment xml:lang="en">A ratio attribute that is plain/proper</rdfs:comment>
    <rdfs:subClassOf rdf:resource="http://geographicknowledge.de/vocab/CoreConceptData.rdf#RatioA" />
    <owl:equivalentClass>
      <owl:Class>
        <owl:intersectionOf rdf:nodeID="autos367" />
      </owl:Class>
    </owl:equivalentClass>
  </owl:Class>
  <owl:Class rdf:about="http://geographicknowledge.de/vocab/CoreConceptData.rdf#PlainVectorRegion">
    <rdfs:comment xml:lang="en">Vector regions that are not tessellated</rdfs:comment>
    <rdfs:subClassOf rdf:resource="http://geographicknowledge.de/vocab/CoreConceptData.rdf#VectorRegion" />
    <owl:equivalentClass>
      <owl:Class>
        <owl:intersectionOf rdf:nodeID="autos371" />
      </owl:Class>
    </owl:equivalentClass>
  </owl:Class>
  <owl:Class rdf:about="http://geographicknowledge.de/vocab/CoreConceptData.rdf#PlainVectorRegionA">
    <rdfs:comment xml:lang="en">An attribute of a vector region layer that is not a tessellation</rdfs:comment>
    <rdfs:subClassOf rdf:resource="http://geographicknowledge.de/vocab/CoreConceptData.rdf#RegionA" />
    <rdfs:subClassOf rdf:resource="http://geographicknowledge.de/vocab/CoreConceptData.rdf#VectorA" />
    <rdfs:subClassOf rdf:resource="http://geographicknowledge.de/vocab/CoreConceptData.rdf#VectorRegionA" />
    <owl:equivalentClass>
      <owl:Class>
        <owl:intersectionOf rdf:nodeID="autos375" />
      </owl:Class>
    </owl:equivalentClass>
  </owl:Class>
  <owl:Class rdf:about="http://geographicknowledge.de/vocab/CoreConceptData.rdf#Point">
    <rdfs:comment xml:lang="en">A generalized notion of a point in 2D and 3D</rdfs:comment>
    <rdfs:subClassOf rdf:resource="http://geographicknowledge.de/vocab/AnalysisData.rdf#Spatial" />
  </owl:Class>
  <owl:Class rdf:about="http://geographicknowledge.de/vocab/CoreConceptData.rdf#PointA">
    <rdfs:comment xml:lang="en">Attribute of some point data set</rdfs:comment>
    <rdfs:subClassOf rdf:resource="http://geographicknowledge.de/vocab/CoreConceptData.rdf#VectorA" />
    <owl:equivalentClass>
      <owl:Class>
        <owl:intersectionOf rdf:nodeID="autos380" />
      </owl:Class>
    </owl:equivalentClass>
  </owl:Class>
  <owl:Class rdf:about="http://geographicknowledge.de/vocab/CoreConceptData.rdf#PointDS">
    <owl:disjointWith rdf:resource="http://geographicknowledge.de/vocab/CoreConceptData.rdf#RegionDS" />
    <owl:equivalentClass>
      <owl:Class>
        <owl:intersectionOf rdf:nodeID="autos384" />
      </owl:Class>
    </owl:equivalentClass>
  </owl:Class>
  <owl:Class rdf:about="http://geographicknowledge.de/vocab/CoreConceptData.rdf#PointData">
    <owl:equivalentClass>
      <owl:Class>
        <owl:intersectionOf rdf:nodeID="autos388" />
      </owl:Class>
    </owl:equivalentClass>
  </owl:Class>
  <owl:Class rdf:about="http://geographicknowledge.de/vocab/CoreConceptData.rdf#PointMeasures">
    <rdfs:comment xml:lang="en">Point measures are point-like representations of fields. For example, point data sets denoting the locations of measured temperature values.</rdfs:comment>
    <rdfs:subClassOf rdf:resource="http://geographicknowledge.de/vocab/CoreConceptData.rdf#FieldQ" />
    <rdfs:subClassOf rdf:resource="http://geographicknowledge.de/vocab/CoreConceptData.rdf#PointA" />
    <owl:equivalentClass>
      <owl:Class>
        <owl:intersectionOf rdf:nodeID="autos392" />
      </owl:Class>
    </owl:equivalentClass>
  </owl:Class>
  <owl:Class rdf:about="http://geographicknowledge.de/vocab/CoreConceptData.rdf#PointMeasuresDS">
    <rdfs:comment xml:lang="en">A dataset representing a field in terms of point-wise measures. For example, temperature sensor measurements.</rdfs:comment>
    <rdfs:subClassOf rdf:resource="http://geographicknowledge.de/vocab/CoreConceptData.rdf#FieldDS" />
    <owl:equivalentClass>
      <owl:Class>
        <owl:intersectionOf rdf:nodeID="autos396" />
      </owl:Class>
    </owl:equivalentClass>
  </owl:Class>
  <owl:Class rdf:about="http://geographicknowledge.de/vocab/CoreConceptData.rdf#QualityValue">
    <rdfs:comment xml:lang="en">A single value of some quality</rdfs:comment>
    <rdfs:subClassOf rdf:resource="http://geographicknowledge.de/vocab/AnalysisData.rdf#Quality" />
  </owl:Class>
  <owl:Class rdf:about="http://geographicknowledge.de/vocab/CoreConceptData.rdf#Raster">
    <rdfs:comment xml:lang="en">A raster data set is a special kind of tessellation, where regions are regular squares.</rdfs:comment>
    <rdfs:subClassOf rdf:resource="http://geographicknowledge.de/vocab/CoreConceptData.rdf#Tessellation" />
  </owl:Class>
  <owl:Class rdf:about="http://geographicknowledge.de/vocab/CoreConceptData.rdf#RasterA">
    <rdfs:comment xml:lang="en">Attribute of some Raster</rdfs:comment>
    <rdfs:subClassOf rdf:resource="http://geographicknowledge.de/vocab/CoreConceptData.rdf#TessellationA" />
    <owl:equivalentClass>
      <owl:Class>
        <owl:intersectionOf rdf:nodeID="autos399" />
      </owl:Class>
    </owl:equivalentClass>
  </owl:Class>
  <owl:Class rdf:about="http://geographicknowledge.de/vocab/CoreConceptData.rdf#RatioA">
    <rdfs:comment xml:lang="en">Spatial attribute on ratio scale level</rdfs:comment>
    <rdfs:subClassOf rdf:resource="http://geographicknowledge.de/vocab/CoreConceptData.rdf#IntervalA" />
  </owl:Class>
  <owl:Class rdf:about="http://geographicknowledge.de/vocab/CoreConceptData.rdf#Region">
    <rdfs:comment xml:lang="en">A generalized geometry, including 2D and 3D extended regions. In 2D, this might be a Polygon.</rdfs:comment>
    <rdfs:subClassOf rdf:resource="http://geographicknowledge.de/vocab/AnalysisData.rdf#Spatial" />
  </owl:Class>
  <owl:Class rdf:about="http://geographicknowledge.de/vocab/CoreConceptData.rdf#RegionA">
    <rdfs:comment xml:lang="en">Atrribute of some region data sets</rdfs:comment>
    <rdfs:subClassOf rdf:resource="http://geographicknowledge.de/vocab/CoreConceptData.rdf#LayerA" />
    <owl:equivalentClass>
      <owl:Class>
        <owl:intersectionOf rdf:nodeID="autos403" />
      </owl:Class>
    </owl:equivalentClass>
  </owl:Class>
  <owl:Class rdf:about="http://geographicknowledge.de/vocab/CoreConceptData.rdf#RegionDS">
    <owl:equivalentClass>
      <owl:Class>
        <owl:intersectionOf rdf:nodeID="autos407" />
      </owl:Class>
    </owl:equivalentClass>
  </owl:Class>
  <owl:Class rdf:about="http://geographicknowledge.de/vocab/CoreConceptData.rdf#RegionData">
    <owl:equivalentClass>
      <owl:Class>
        <owl:intersectionOf rdf:nodeID="autos411" />
      </owl:Class>
    </owl:equivalentClass>
  </owl:Class>
  <owl:Class rdf:about="http://geographicknowledge.de/vocab/CoreConceptData.rdf#RelationalDS">
    <rdfs:comment xml:lang="en">A dataset that represents some quantified realtionb between other concepts. For example, a network (being a relation between objects).</rdfs:comment>
    <rdfs:subClassOf rdf:resource="http://geographicknowledge.de/vocab/CoreConceptData.rdf#CoreConceptDataSet" />
  </owl:Class>
  <owl:Class rdf:about="http://geographicknowledge.de/vocab/CoreConceptData.rdf#RelationalQ">
    <rdfs:comment xml:lang="en">An attribute of a dataset that represents some quantified relation between other core concepts. For example a network is relation between objects.</rdfs:comment>
    <rdfs:subClassOf rdf:resource="http://geographicknowledge.de/vocab/CoreConceptData.rdf#CoreConceptQ" />
    <owl:equivalentClass>
      <owl:Restriction>
        <owl:onProperty rdf:resource="http://geographicknowledge.de/vocab/AnalysisData.rdf#ofDataSet" />
        <owl:someValuesFrom rdf:resource="http://geographicknowledge.de/vocab/CoreConceptData.rdf#RelationalDS" />
      </owl:Restriction>
    </owl:equivalentClass>
  </owl:Class>
  <owl:Class rdf:about="http://geographicknowledge.de/vocab/CoreConceptData.rdf#Tessellation">
    <rdfs:comment xml:lang="en">A region data set where spatial regions are tessellated (jointly covering and mutually non-overlapping) within a spatial extent</rdfs:comment>
    <rdfs:subClassOf rdf:resource="http://geographicknowledge.de/vocab/CoreConceptData.rdf#RegionDS" />
  </owl:Class>
  <owl:Class rdf:about="http://geographicknowledge.de/vocab/CoreConceptData.rdf#TessellationA">
    <rdfs:comment xml:lang="en">An attribute of a tesselation data set</rdfs:comment>
    <rdfs:subClassOf rdf:resource="http://geographicknowledge.de/vocab/CoreConceptData.rdf#RegionA" />
    <owl:equivalentClass>
      <owl:Class>
        <owl:intersectionOf rdf:nodeID="autos416" />
      </owl:Class>
    </owl:equivalentClass>
  </owl:Class>
  <owl:Class rdf:about="http://geographicknowledge.de/vocab/CoreConceptData.rdf#Track">
    <rdfs:comment xml:lang="en">A type for a spatial track. A spatial track is a vector representation of "fix" events of some moving object. For example, a GPS track of points of a person moving.</rdfs:comment>
    <rdfs:subClassOf rdf:resource="http://geographicknowledge.de/vocab/CoreConceptData.rdf#EventVector" />
  </owl:Class>
  <owl:Class rdf:about="http://geographicknowledge.de/vocab/CoreConceptData.rdf#TrackDS">
    <rdfs:comment xml:lang="en">A dataset representing tracks, i.e. point wise events (fixes) of the trajectory of some objects.</rdfs:comment>
    <rdfs:subClassOf rdf:resource="http://geographicknowledge.de/vocab/CoreConceptData.rdf#EventDS" />
    <rdfs:subClassOf rdf:resource="http://geographicknowledge.de/vocab/CoreConceptData.rdf#PointDS" />
  </owl:Class>
  <owl:Class rdf:about="http://geographicknowledge.de/vocab/CoreConceptData.rdf#Vector">
    <rdfs:comment xml:lang="en">Vector data sets are spatial data sets that are not raster</rdfs:comment>
    <owl:equivalentClass>
      <owl:Class>
        <owl:intersectionOf rdf:nodeID="autos420" />
      </owl:Class>
    </owl:equivalentClass>
  </owl:Class>
  <owl:Class rdf:about="http://geographicknowledge.de/vocab/CoreConceptData.rdf#VectorA">
    <rdfs:comment xml:lang="en">Attribute of some vector data set</rdfs:comment>
    <rdfs:subClassOf rdf:resource="http://geographicknowledge.de/vocab/CoreConceptData.rdf#LayerA" />
    <owl:equivalentClass>
      <owl:Class>
        <owl:intersectionOf rdf:nodeID="autos424" />
      </owl:Class>
    </owl:equivalentClass>
  </owl:Class>
  <owl:Class rdf:about="http://geographicknowledge.de/vocab/CoreConceptData.rdf#VectorRegion">
    <rdfs:comment xml:lang="en">Dataset with vector regions as geometry</rdfs:comment>
    <rdfs:subClassOf rdf:resource="http://geographicknowledge.de/vocab/CoreConceptData.rdf#RegionDS" />
    <rdfs:subClassOf rdf:resource="http://geographicknowledge.de/vocab/CoreConceptData.rdf#Vector" />
    <owl:equivalentClass>
      <owl:Class>
        <owl:intersectionOf rdf:nodeID="autos428" />
      </owl:Class>
    </owl:equivalentClass>
  </owl:Class>
  <owl:Class rdf:about="http://geographicknowledge.de/vocab/CoreConceptData.rdf#VectorRegionA">
    <rdfs:comment xml:lang="en">An attribute of a region vector layer</rdfs:comment>
    <rdfs:subClassOf rdf:resource="http://geographicknowledge.de/vocab/CoreConceptData.rdf#RegionA" />
    <rdfs:subClassOf rdf:resource="http://geographicknowledge.de/vocab/CoreConceptData.rdf#VectorA" />
    <owl:equivalentClass>
      <owl:Class>
        <owl:intersectionOf rdf:nodeID="autos431" />
      </owl:Class>
    </owl:equivalentClass>
  </owl:Class>
  <owl:Class rdf:about="http://geographicknowledge.de/vocab/CoreConceptData.rdf#VectorTessellation">
    <rdfs:comment xml:lang="en">This is a vector data set which is tessellated (and no raster)</rdfs:comment>
    <rdfs:subClassOf rdf:resource="http://geographicknowledge.de/vocab/CoreConceptData.rdf#Tessellation" />
    <rdfs:subClassOf rdf:resource="http://geographicknowledge.de/vocab/CoreConceptData.rdf#VectorRegion" />
    <owl:equivalentClass>
      <owl:Class>
        <owl:intersectionOf rdf:nodeID="autos434" />
      </owl:Class>
    </owl:equivalentClass>
  </owl:Class>
  <owl:Class rdf:about="http://geographicknowledge.de/vocab/CoreConceptData.rdf#VectorTessellationA">
    <rdfs:comment xml:lang="en">An attribute of a vector tessellation</rdfs:comment>
    <rdfs:subClassOf rdf:resource="http://geographicknowledge.de/vocab/CoreConceptData.rdf#TessellationA" />
    <rdfs:subClassOf rdf:resource="http://geographicknowledge.de/vocab/CoreConceptData.rdf#VectorA" />
    <rdfs:subClassOf rdf:resource="http://geographicknowledge.de/vocab/CoreConceptData.rdf#VectorRegionA" />
    <owl:equivalentClass>
      <owl:Class>
        <owl:intersectionOf rdf:nodeID="autos437" />
      </owl:Class>
    </owl:equivalentClass>
  </owl:Class>
  <owl:Class rdf:about="http://geographicknowledge.de/vocab/CoreConceptData.rdf#ZeroExistenceRaster">
    <rdfs:comment xml:lang="en">A raster dataset where 0 is interpreted as boolean "false"</rdfs:comment>
    <rdfs:subClassOf rdf:resource="http://geographicknowledge.de/vocab/CoreConceptData.rdf#ExistenceRaster" />
  </owl:Class>
  <owl:Class rdf:about="http://geographicknowledge.de/vocab/ExtensiveMeasures.rdf#ERA">
    <rdfs:comment xml:lang="en">Extensive region attribute. Since attributes are extensive, their values increase with the size of their support regions. Zero size regions are zero then defined to be zero, which implies a ratio scale level.</rdfs:comment>
    <rdfs:subClassOf rdf:resource="http://geographicknowledge.de/vocab/CoreConceptData.rdf#RatioA" />
  </owl:Class>
  <owl:Class rdf:about="http://geographicknowledge.de/vocab/ExtensiveMeasures.rdf#IRA">
    <rdfs:comment xml:lang="en">Intensive region attribute. An attribute that is independent from the size of its support region.</rdfs:comment>
    <rdfs:subClassOf rdf:resource="http://geographicknowledge.de/vocab/CoreConceptData.rdf#RatioA" />
  </owl:Class>
  <owl:ObjectProperty rdf:about="http://geographicknowledge.de/vocab/GISConcepts.rdf#hasAttribute" />
  <rdf:Description rdf:nodeID="autos260">
    <rdf:first rdf:resource="http://geographicknowledge.de/vocab/CoreConceptData.rdf#AmountDS" />
    <rdf:rest rdf:nodeID="autos261" />
  </rdf:Description>
  <rdf:Description rdf:nodeID="autos261">
    <rdf:first rdf:resource="http://geographicknowledge.de/vocab/CoreConceptData.rdf#Raster" />
    <rdf:rest rdf:resource="http://www.w3.org/1999/02/22-rdf-syntax-ns#nil" />
  </rdf:Description>
  <rdf:Description rdf:nodeID="autos263">
    <rdf:first rdf:resource="http://geographicknowledge.de/vocab/CoreConceptData.rdf#AmountDS" />
    <rdf:rest rdf:nodeID="autos264" />
  </rdf:Description>
  <rdf:Description rdf:nodeID="autos264">
    <rdf:first rdf:resource="http://geographicknowledge.de/vocab/CoreConceptData.rdf#Vector" />
    <rdf:rest rdf:resource="http://www.w3.org/1999/02/22-rdf-syntax-ns#nil" />
  </rdf:Description>
  <rdf:Description rdf:nodeID="autos266">
    <rdf:first rdf:resource="http://geographicknowledge.de/vocab/CoreConceptData.rdf#ExistenceRaster" />
    <rdf:rest rdf:nodeID="autos267" />
  </rdf:Description>
  <rdf:Description rdf:nodeID="autos267">
    <rdf:first rdf:resource="http://geographicknowledge.de/vocab/CoreConceptData.rdf#ExistenceVector" />
    <rdf:rest rdf:nodeID="autos268" />
  </rdf:Description>
  <rdf:Description rdf:nodeID="autos268">
    <rdf:first rdf:resource="http://geographicknowledge.de/vocab/CoreConceptData.rdf#ObjectVector" />
    <rdf:rest rdf:resource="http://www.w3.org/1999/02/22-rdf-syntax-ns#nil" />
  </rdf:Description>
  <rdf:Description rdf:nodeID="autos270">
    <rdf:first rdf:resource="http://geographicknowledge.de/vocab/CoreConceptData.rdf#FieldQ" />
    <rdf:rest rdf:nodeID="autos271" />
  </rdf:Description>
  <rdf:Description rdf:nodeID="autos271">
    <rdf:first>
      <owl:Restriction>
        <owl:onProperty rdf:resource="http://geographicknowledge.de/vocab/AnalysisData.rdf#ofDataSet" />
        <owl:someValuesFrom rdf:resource="http://geographicknowledge.de/vocab/CoreConceptData.rdf#Tessellation" />
      </owl:Restriction>
    </rdf:first>
    <rdf:rest rdf:resource="http://www.w3.org/1999/02/22-rdf-syntax-ns#nil" />
  </rdf:Description>
  <rdf:Description rdf:nodeID="autos274">
    <rdf:first rdf:resource="http://geographicknowledge.de/vocab/CoreConceptData.rdf#FieldDS" />
    <rdf:rest rdf:nodeID="autos275" />
  </rdf:Description>
  <rdf:Description rdf:nodeID="autos275">
    <rdf:first rdf:resource="http://geographicknowledge.de/vocab/CoreConceptData.rdf#Tessellation" />
    <rdf:rest rdf:resource="http://www.w3.org/1999/02/22-rdf-syntax-ns#nil" />
  </rdf:Description>
  <rdf:Description rdf:nodeID="autos278">
    <rdf:first rdf:resource="http://geographicknowledge.de/vocab/CoreConceptData.rdf#EventQ" />
    <rdf:rest rdf:nodeID="autos279" />
  </rdf:Description>
  <rdf:Description rdf:nodeID="autos279">
    <rdf:first>
      <owl:Restriction>
        <owl:onProperty rdf:resource="http://geographicknowledge.de/vocab/AnalysisData.rdf#ofDataSet" />
        <owl:someValuesFrom rdf:resource="http://geographicknowledge.de/vocab/CoreConceptData.rdf#Vector" />
      </owl:Restriction>
    </rdf:first>
    <rdf:rest rdf:resource="http://www.w3.org/1999/02/22-rdf-syntax-ns#nil" />
  </rdf:Description>
  <rdf:Description rdf:nodeID="autos282">
    <rdf:first rdf:resource="http://geographicknowledge.de/vocab/CoreConceptData.rdf#BooleanA" />
    <rdf:rest rdf:nodeID="autos283" />
  </rdf:Description>
  <rdf:Description rdf:nodeID="autos283">
    <rdf:first rdf:resource="http://geographicknowledge.de/vocab/CoreConceptData.rdf#FieldRaster" />
    <rdf:rest rdf:resource="http://www.w3.org/1999/02/22-rdf-syntax-ns#nil" />
  </rdf:Description>
  <rdf:Description rdf:nodeID="autos285">
    <rdf:first rdf:resource="http://geographicknowledge.de/vocab/CoreConceptData.rdf#BooleanA" />
    <rdf:rest rdf:nodeID="autos286" />
  </rdf:Description>
  <rdf:Description rdf:nodeID="autos286">
    <rdf:first rdf:resource="http://geographicknowledge.de/vocab/CoreConceptData.rdf#FieldVector" />
    <rdf:rest rdf:resource="http://www.w3.org/1999/02/22-rdf-syntax-ns#nil" />
  </rdf:Description>
  <rdf:Description rdf:nodeID="autos288">
    <rdf:first rdf:resource="http://geographicknowledge.de/vocab/CoreConceptData.rdf#Lattice" />
    <rdf:rest rdf:nodeID="autos289" />
  </rdf:Description>
  <rdf:Description rdf:nodeID="autos289">
    <rdf:first rdf:resource="http://geographicknowledge.de/vocab/ExtensiveMeasures.rdf#ERA" />
    <rdf:rest rdf:resource="http://www.w3.org/1999/02/22-rdf-syntax-ns#nil" />
  </rdf:Description>
  <rdf:Description rdf:nodeID="autos292">
    <rdf:first rdf:resource="http://geographicknowledge.de/vocab/CoreConceptData.rdf#FieldQ" />
    <rdf:rest rdf:nodeID="autos293" />
  </rdf:Description>
  <rdf:Description rdf:nodeID="autos293">
    <rdf:first>
      <owl:Restriction>
        <owl:onProperty rdf:resource="http://geographicknowledge.de/vocab/AnalysisData.rdf#ofDataSet" />
        <owl:someValuesFrom rdf:resource="http://geographicknowledge.de/vocab/CoreConceptData.rdf#Raster" />
      </owl:Restriction>
    </rdf:first>
    <rdf:rest rdf:resource="http://www.w3.org/1999/02/22-rdf-syntax-ns#nil" />
  </rdf:Description>
  <rdf:Description rdf:nodeID="autos296">
    <rdf:first rdf:resource="http://geographicknowledge.de/vocab/CoreConceptData.rdf#FieldDS" />
    <rdf:rest rdf:nodeID="autos297" />
  </rdf:Description>
  <rdf:Description rdf:nodeID="autos297">
    <rdf:first rdf:resource="http://geographicknowledge.de/vocab/CoreConceptData.rdf#Raster" />
    <rdf:rest rdf:resource="http://www.w3.org/1999/02/22-rdf-syntax-ns#nil" />
  </rdf:Description>
  <rdf:Description rdf:nodeID="autos299">
    <rdf:first rdf:resource="http://geographicknowledge.de/vocab/CoreConceptData.rdf#FieldQ" />
    <rdf:rest rdf:nodeID="autos300" />
  </rdf:Description>
  <rdf:Description rdf:nodeID="autos300">
    <rdf:first>
      <owl:Restriction>
        <owl:onProperty rdf:resource="http://geographicknowledge.de/vocab/AnalysisData.rdf#ofDataSet" />
        <owl:someValuesFrom rdf:resource="http://geographicknowledge.de/vocab/CoreConceptData.rdf#Vector" />
      </owl:Restriction>
    </rdf:first>
    <rdf:rest rdf:resource="http://www.w3.org/1999/02/22-rdf-syntax-ns#nil" />
  </rdf:Description>
  <rdf:Description rdf:nodeID="autos303">
    <rdf:first rdf:resource="http://geographicknowledge.de/vocab/CoreConceptData.rdf#ObjectQ" />
    <rdf:rest rdf:nodeID="autos304" />
  </rdf:Description>
  <rdf:Description rdf:nodeID="autos304">
    <rdf:first>
      <owl:Restriction>
        <owl:onProperty rdf:resource="http://geographicknowledge.de/vocab/AnalysisData.rdf#ofDataSet" />
        <owl:someValuesFrom rdf:resource="http://geographicknowledge.de/vocab/CoreConceptData.rdf#Tessellation" />
      </owl:Restriction>
    </rdf:first>
    <rdf:rest rdf:resource="http://www.w3.org/1999/02/22-rdf-syntax-ns#nil" />
  </rdf:Description>
  <rdf:Description rdf:nodeID="autos307">
    <rdf:first rdf:resource="http://geographicknowledge.de/vocab/CoreConceptData.rdf#ObjectDS" />
    <rdf:rest rdf:nodeID="autos308" />
  </rdf:Description>
  <rdf:Description rdf:nodeID="autos308">
    <rdf:first rdf:resource="http://geographicknowledge.de/vocab/CoreConceptData.rdf#Tessellation" />
    <rdf:rest rdf:resource="http://www.w3.org/1999/02/22-rdf-syntax-ns#nil" />
  </rdf:Description>
  <rdf:Description rdf:nodeID="autos310">
    <rdf:first rdf:resource="http://geographicknowledge.de/vocab/CoreConceptData.rdf#Attribute" />
    <rdf:rest rdf:nodeID="autos311" />
  </rdf:Description>
  <rdf:Description rdf:nodeID="autos311">
    <rdf:first>
      <owl:Restriction>
        <owl:onProperty rdf:resource="http://geographicknowledge.de/vocab/AnalysisData.rdf#ofDataSet" />
        <owl:someValuesFrom rdf:resource="http://geographicknowledge.de/vocab/CoreConceptData.rdf#LineDS" />
      </owl:Restriction>
    </rdf:first>
    <rdf:rest rdf:resource="http://www.w3.org/1999/02/22-rdf-syntax-ns#nil" />
  </rdf:Description>
  <rdf:Description rdf:nodeID="autos314">
    <rdf:first rdf:resource="http://geographicknowledge.de/vocab/CoreConceptData.rdf#Vector" />
    <rdf:rest rdf:nodeID="autos315" />
  </rdf:Description>
  <rdf:Description rdf:nodeID="autos315">
    <rdf:first>
      <owl:Restriction>
        <owl:onProperty rdf:resource="http://geographicknowledge.de/vocab/AnalysisData.rdf#hasElement" />
        <owl:allValuesFrom rdf:resource="http://geographicknowledge.de/vocab/CoreConceptData.rdf#LineData" />
      </owl:Restriction>
    </rdf:first>
    <rdf:rest rdf:resource="http://www.w3.org/1999/02/22-rdf-syntax-ns#nil" />
  </rdf:Description>
  <rdf:Description rdf:nodeID="autos318">
    <rdf:first rdf:resource="http://geographicknowledge.de/vocab/AnalysisData.rdf#SpatialData" />
    <rdf:rest rdf:nodeID="autos319" />
  </rdf:Description>
  <rdf:Description rdf:nodeID="autos319">
    <rdf:first>
      <owl:Restriction>
        <owl:onProperty rdf:resource="http://geographicknowledge.de/vocab/GISConcepts.rdf#hasAttribute" />
        <owl:someValuesFrom rdf:resource="http://geographicknowledge.de/vocab/CoreConceptData.rdf#Line" />
      </owl:Restriction>
    </rdf:first>
    <rdf:rest rdf:resource="http://www.w3.org/1999/02/22-rdf-syntax-ns#nil" />
  </rdf:Description>
  <rdf:Description rdf:nodeID="autos322">
    <rdf:first rdf:resource="http://geographicknowledge.de/vocab/CoreConceptData.rdf#FieldQ" />
    <rdf:rest rdf:nodeID="autos323" />
  </rdf:Description>
  <rdf:Description rdf:nodeID="autos323">
    <rdf:first>
      <owl:Restriction>
        <owl:onProperty rdf:resource="http://geographicknowledge.de/vocab/AnalysisData.rdf#ofDataSet" />
        <owl:someValuesFrom rdf:resource="http://geographicknowledge.de/vocab/CoreConceptData.rdf#LineDS" />
      </owl:Restriction>
    </rdf:first>
    <rdf:rest rdf:resource="http://www.w3.org/1999/02/22-rdf-syntax-ns#nil" />
  </rdf:Description>
  <rdf:Description rdf:nodeID="autos326">
    <rdf:first rdf:resource="http://geographicknowledge.de/vocab/CoreConceptData.rdf#FieldDS" />
    <rdf:rest rdf:nodeID="autos327" />
  </rdf:Description>
  <rdf:Description rdf:nodeID="autos327">
    <rdf:first rdf:resource="http://geographicknowledge.de/vocab/CoreConceptData.rdf#LineDS" />
    <rdf:rest rdf:resource="http://www.w3.org/1999/02/22-rdf-syntax-ns#nil" />
  </rdf:Description>
  <rdf:Description rdf:nodeID="autos331">
    <rdf:first rdf:resource="http://geographicknowledge.de/vocab/CoreConceptData.rdf#ObjectQ" />
    <rdf:rest rdf:nodeID="autos332" />
  </rdf:Description>
  <rdf:Description rdf:nodeID="autos332">
    <rdf:first>
      <owl:Restriction>
        <owl:onProperty rdf:resource="http://geographicknowledge.de/vocab/AnalysisData.rdf#ofDataSet" />
        <owl:someValuesFrom rdf:resource="http://geographicknowledge.de/vocab/CoreConceptData.rdf#LineDS" />
      </owl:Restriction>
    </rdf:first>
    <rdf:rest rdf:resource="http://www.w3.org/1999/02/22-rdf-syntax-ns#nil" />
  </rdf:Description>
  <rdf:Description rdf:nodeID="autos335">
    <rdf:first rdf:resource="http://geographicknowledge.de/vocab/CoreConceptData.rdf#ObjectQ" />
    <rdf:rest rdf:nodeID="autos336" />
  </rdf:Description>
  <rdf:Description rdf:nodeID="autos336">
    <rdf:first>
      <owl:Restriction>
        <owl:onProperty rdf:resource="http://geographicknowledge.de/vocab/AnalysisData.rdf#ofDataSet" />
        <owl:someValuesFrom rdf:resource="http://geographicknowledge.de/vocab/CoreConceptData.rdf#PointDS" />
      </owl:Restriction>
    </rdf:first>
    <rdf:rest rdf:resource="http://www.w3.org/1999/02/22-rdf-syntax-ns#nil" />
  </rdf:Description>
  <rdf:Description rdf:nodeID="autos340">
    <rdf:first rdf:resource="http://geographicknowledge.de/vocab/CoreConceptData.rdf#ObjectQ" />
    <rdf:rest rdf:nodeID="autos341" />
  </rdf:Description>
  <rdf:Description rdf:nodeID="autos341">
    <rdf:first>
      <owl:Restriction>
        <owl:onProperty rdf:resource="http://geographicknowledge.de/vocab/AnalysisData.rdf#ofDataSet" />
        <owl:someValuesFrom rdf:resource="http://geographicknowledge.de/vocab/CoreConceptData.rdf#RegionDS" />
      </owl:Restriction>
    </rdf:first>
    <rdf:rest rdf:resource="http://www.w3.org/1999/02/22-rdf-syntax-ns#nil" />
  </rdf:Description>
  <rdf:Description rdf:nodeID="autos344">
    <rdf:first rdf:resource="http://geographicknowledge.de/vocab/CoreConceptData.rdf#ObjectQ" />
    <rdf:rest rdf:nodeID="autos345" />
  </rdf:Description>
  <rdf:Description rdf:nodeID="autos345">
    <rdf:first>
      <owl:Restriction>
        <owl:onProperty rdf:resource="http://geographicknowledge.de/vocab/AnalysisData.rdf#ofDataSet" />
        <owl:someValuesFrom rdf:resource="http://geographicknowledge.de/vocab/CoreConceptData.rdf#Vector" />
      </owl:Restriction>
    </rdf:first>
    <rdf:rest rdf:resource="http://www.w3.org/1999/02/22-rdf-syntax-ns#nil" />
  </rdf:Description>
  <rdf:Description rdf:nodeID="autos348">
    <rdf:first rdf:resource="http://geographicknowledge.de/vocab/CoreConceptData.rdf#FieldQ" />
    <rdf:rest rdf:nodeID="autos349" />
  </rdf:Description>
  <rdf:Description rdf:nodeID="autos349">
    <rdf:first>
      <owl:Restriction>
        <owl:onProperty rdf:resource="http://geographicknowledge.de/vocab/AnalysisData.rdf#ofDataSet" />
        <owl:someValuesFrom rdf:resource="http://geographicknowledge.de/vocab/CoreConceptData.rdf#RegionDS" />
      </owl:Restriction>
    </rdf:first>
    <rdf:rest rdf:resource="http://www.w3.org/1999/02/22-rdf-syntax-ns#nil" />
  </rdf:Description>
  <rdf:Description rdf:nodeID="autos352">
    <rdf:first rdf:resource="http://geographicknowledge.de/vocab/CoreConceptData.rdf#FieldDS" />
    <rdf:rest rdf:nodeID="autos353" />
  </rdf:Description>
  <rdf:Description rdf:nodeID="autos353">
    <rdf:first rdf:resource="http://geographicknowledge.de/vocab/CoreConceptData.rdf#RegionDS" />
    <rdf:rest rdf:resource="http://www.w3.org/1999/02/22-rdf-syntax-ns#nil" />
  </rdf:Description>
  <rdf:Description rdf:nodeID="autos355">
    <rdf:first rdf:resource="http://geographicknowledge.de/vocab/CoreConceptData.rdf#IntervalA" />
    <rdf:rest rdf:nodeID="autos356" />
  </rdf:Description>
  <rdf:Description rdf:nodeID="autos356">
    <rdf:first>
      <owl:Class>
        <owl:complementOf rdf:resource="http://geographicknowledge.de/vocab/CoreConceptData.rdf#RatioA" />
      </owl:Class>
    </rdf:first>
    <rdf:rest rdf:resource="http://www.w3.org/1999/02/22-rdf-syntax-ns#nil" />
  </rdf:Description>
  <rdf:Description rdf:nodeID="autos359">
    <rdf:first rdf:resource="http://geographicknowledge.de/vocab/CoreConceptData.rdf#NominalA" />
    <rdf:rest rdf:nodeID="autos360" />
  </rdf:Description>
  <rdf:Description rdf:nodeID="autos360">
    <rdf:first>
      <owl:Class>
        <owl:complementOf rdf:resource="http://geographicknowledge.de/vocab/CoreConceptData.rdf#OrdinalA" />
      </owl:Class>
    </rdf:first>
    <rdf:rest rdf:resource="http://www.w3.org/1999/02/22-rdf-syntax-ns#nil" />
  </rdf:Description>
  <rdf:Description rdf:nodeID="autos363">
    <rdf:first rdf:resource="http://geographicknowledge.de/vocab/CoreConceptData.rdf#OrdinalA" />
    <rdf:rest rdf:nodeID="autos364" />
  </rdf:Description>
  <rdf:Description rdf:nodeID="autos364">
    <rdf:first>
      <owl:Class>
        <owl:complementOf rdf:resource="http://geographicknowledge.de/vocab/CoreConceptData.rdf#IntervalA" />
      </owl:Class>
    </rdf:first>
    <rdf:rest rdf:resource="http://www.w3.org/1999/02/22-rdf-syntax-ns#nil" />
  </rdf:Description>
  <rdf:Description rdf:nodeID="autos367">
    <rdf:first rdf:resource="http://geographicknowledge.de/vocab/CoreConceptData.rdf#RatioA" />
    <rdf:rest rdf:nodeID="autos368" />
  </rdf:Description>
  <rdf:Description rdf:nodeID="autos368">
    <rdf:first>
      <owl:Class>
        <owl:complementOf rdf:resource="http://geographicknowledge.de/vocab/CoreConceptData.rdf#CountA" />
      </owl:Class>
    </rdf:first>
    <rdf:rest rdf:resource="http://www.w3.org/1999/02/22-rdf-syntax-ns#nil" />
  </rdf:Description>
  <rdf:Description rdf:nodeID="autos371">
    <rdf:first rdf:resource="http://geographicknowledge.de/vocab/CoreConceptData.rdf#VectorRegion" />
    <rdf:rest rdf:nodeID="autos372" />
  </rdf:Description>
  <rdf:Description rdf:nodeID="autos372">
    <rdf:first>
      <owl:Class>
        <owl:complementOf rdf:resource="http://geographicknowledge.de/vocab/CoreConceptData.rdf#Tessellation" />
      </owl:Class>
    </rdf:first>
    <rdf:rest rdf:resource="http://www.w3.org/1999/02/22-rdf-syntax-ns#nil" />
  </rdf:Description>
  <rdf:Description rdf:nodeID="autos375">
    <rdf:first rdf:resource="http://geographicknowledge.de/vocab/CoreConceptData.rdf#RegionA" />
    <rdf:rest rdf:nodeID="autos376" />
  </rdf:Description>
  <rdf:Description rdf:nodeID="autos376">
    <rdf:first rdf:resource="http://geographicknowledge.de/vocab/CoreConceptData.rdf#VectorA" />
    <rdf:rest rdf:nodeID="autos377" />
  </rdf:Description>
  <rdf:Description rdf:nodeID="autos377">
    <rdf:first>
      <owl:Class>
        <owl:complementOf rdf:resource="http://geographicknowledge.de/vocab/CoreConceptData.rdf#TessellationA" />
      </owl:Class>
    </rdf:first>
    <rdf:rest rdf:resource="http://www.w3.org/1999/02/22-rdf-syntax-ns#nil" />
  </rdf:Description>
  <rdf:Description rdf:nodeID="autos380">
    <rdf:first rdf:resource="http://geographicknowledge.de/vocab/CoreConceptData.rdf#Attribute" />
    <rdf:rest rdf:nodeID="autos381" />
  </rdf:Description>
  <rdf:Description rdf:nodeID="autos381">
    <rdf:first>
      <owl:Restriction>
        <owl:onProperty rdf:resource="http://geographicknowledge.de/vocab/AnalysisData.rdf#ofDataSet" />
        <owl:someValuesFrom rdf:resource="http://geographicknowledge.de/vocab/CoreConceptData.rdf#PointDS" />
      </owl:Restriction>
    </rdf:first>
    <rdf:rest rdf:resource="http://www.w3.org/1999/02/22-rdf-syntax-ns#nil" />
  </rdf:Description>
  <rdf:Description rdf:nodeID="autos384">
    <rdf:first rdf:resource="http://geographicknowledge.de/vocab/CoreConceptData.rdf#Vector" />
    <rdf:rest rdf:nodeID="autos385" />
  </rdf:Description>
  <rdf:Description rdf:nodeID="autos385">
    <rdf:first>
      <owl:Restriction>
        <owl:onProperty rdf:resource="http://geographicknowledge.de/vocab/AnalysisData.rdf#hasElement" />
        <owl:allValuesFrom rdf:resource="http://geographicknowledge.de/vocab/CoreConceptData.rdf#PointData" />
      </owl:Restriction>
    </rdf:first>
    <rdf:rest rdf:resource="http://www.w3.org/1999/02/22-rdf-syntax-ns#nil" />
  </rdf:Description>
  <rdf:Description rdf:nodeID="autos388">
    <rdf:first rdf:resource="http://geographicknowledge.de/vocab/AnalysisData.rdf#SpatialData" />
    <rdf:rest rdf:nodeID="autos389" />
  </rdf:Description>
  <rdf:Description rdf:nodeID="autos389">
    <rdf:first>
      <owl:Restriction>
        <owl:onProperty rdf:resource="http://geographicknowledge.de/vocab/GISConcepts.rdf#hasAttribute" />
        <owl:someValuesFrom rdf:resource="http://geographicknowledge.de/vocab/CoreConceptData.rdf#Point" />
      </owl:Restriction>
    </rdf:first>
    <rdf:rest rdf:resource="http://www.w3.org/1999/02/22-rdf-syntax-ns#nil" />
  </rdf:Description>
  <rdf:Description rdf:nodeID="autos392">
    <rdf:first rdf:resource="http://geographicknowledge.de/vocab/CoreConceptData.rdf#FieldQ" />
    <rdf:rest rdf:nodeID="autos393" />
  </rdf:Description>
  <rdf:Description rdf:nodeID="autos393">
    <rdf:first>
      <owl:Restriction>
        <owl:onProperty rdf:resource="http://geographicknowledge.de/vocab/AnalysisData.rdf#ofDataSet" />
        <owl:someValuesFrom rdf:resource="http://geographicknowledge.de/vocab/CoreConceptData.rdf#PointDS" />
      </owl:Restriction>
    </rdf:first>
    <rdf:rest rdf:resource="http://www.w3.org/1999/02/22-rdf-syntax-ns#nil" />
  </rdf:Description>
  <rdf:Description rdf:nodeID="autos396">
    <rdf:first rdf:resource="http://geographicknowledge.de/vocab/CoreConceptData.rdf#FieldDS" />
    <rdf:rest rdf:nodeID="autos397" />
  </rdf:Description>
  <rdf:Description rdf:nodeID="autos397">
    <rdf:first rdf:resource="http://geographicknowledge.de/vocab/CoreConceptData.rdf#PointDS" />
    <rdf:rest rdf:resource="http://www.w3.org/1999/02/22-rdf-syntax-ns#nil" />
  </rdf:Description>
  <rdf:Description rdf:nodeID="autos399">
    <rdf:first rdf:resource="http://geographicknowledge.de/vocab/CoreConceptData.rdf#Attribute" />
    <rdf:rest rdf:nodeID="autos400" />
  </rdf:Description>
  <rdf:Description rdf:nodeID="autos400">
    <rdf:first>
      <owl:Restriction>
        <owl:onProperty rdf:resource="http://geographicknowledge.de/vocab/AnalysisData.rdf#ofDataSet" />
        <owl:someValuesFrom rdf:resource="http://geographicknowledge.de/vocab/CoreConceptData.rdf#Raster" />
      </owl:Restriction>
    </rdf:first>
    <rdf:rest rdf:resource="http://www.w3.org/1999/02/22-rdf-syntax-ns#nil" />
  </rdf:Description>
  <rdf:Description rdf:nodeID="autos403">
    <rdf:first rdf:resource="http://geographicknowledge.de/vocab/CoreConceptData.rdf#Attribute" />
    <rdf:rest rdf:nodeID="autos404" />
  </rdf:Description>
  <rdf:Description rdf:nodeID="autos404">
    <rdf:first>
      <owl:Restriction>
        <owl:onProperty rdf:resource="http://geographicknowledge.de/vocab/AnalysisData.rdf#ofDataSet" />
        <owl:someValuesFrom rdf:resource="http://geographicknowledge.de/vocab/CoreConceptData.rdf#RegionDS" />
      </owl:Restriction>
    </rdf:first>
    <rdf:rest rdf:resource="http://www.w3.org/1999/02/22-rdf-syntax-ns#nil" />
  </rdf:Description>
  <rdf:Description rdf:nodeID="autos407">
    <rdf:first rdf:resource="http://geographicknowledge.de/vocab/AnalysisData.rdf#SpatialDataSet" />
    <rdf:rest rdf:nodeID="autos408" />
  </rdf:Description>
  <rdf:Description rdf:nodeID="autos408">
    <rdf:first>
      <owl:Restriction>
        <owl:onProperty rdf:resource="http://geographicknowledge.de/vocab/AnalysisData.rdf#hasElement" />
        <owl:allValuesFrom rdf:resource="http://geographicknowledge.de/vocab/CoreConceptData.rdf#RegionData" />
      </owl:Restriction>
    </rdf:first>
    <rdf:rest rdf:resource="http://www.w3.org/1999/02/22-rdf-syntax-ns#nil" />
  </rdf:Description>
  <rdf:Description rdf:nodeID="autos411">
    <rdf:first rdf:resource="http://geographicknowledge.de/vocab/AnalysisData.rdf#SpatialData" />
    <rdf:rest rdf:nodeID="autos412" />
  </rdf:Description>
  <rdf:Description rdf:nodeID="autos412">
    <rdf:first>
      <owl:Restriction>
        <owl:onProperty rdf:resource="http://geographicknowledge.de/vocab/GISConcepts.rdf#hasAttribute" />
        <owl:someValuesFrom rdf:resource="http://geographicknowledge.de/vocab/CoreConceptData.rdf#Region" />
      </owl:Restriction>
    </rdf:first>
    <rdf:rest rdf:resource="http://www.w3.org/1999/02/22-rdf-syntax-ns#nil" />
  </rdf:Description>
  <rdf:Description rdf:nodeID="autos416">
    <rdf:first rdf:resource="http://geographicknowledge.de/vocab/CoreConceptData.rdf#Attribute" />
    <rdf:rest rdf:nodeID="autos417" />
  </rdf:Description>
  <rdf:Description rdf:nodeID="autos417">
    <rdf:first>
      <owl:Restriction>
        <owl:onProperty rdf:resource="http://geographicknowledge.de/vocab/AnalysisData.rdf#ofDataSet" />
        <owl:someValuesFrom rdf:resource="http://geographicknowledge.de/vocab/CoreConceptData.rdf#Tessellation" />
      </owl:Restriction>
    </rdf:first>
    <rdf:rest rdf:resource="http://www.w3.org/1999/02/22-rdf-syntax-ns#nil" />
  </rdf:Description>
  <rdf:Description rdf:nodeID="autos420">
    <rdf:first rdf:resource="http://geographicknowledge.de/vocab/AnalysisData.rdf#SpatialDataSet" />
    <rdf:rest rdf:nodeID="autos421" />
  </rdf:Description>
  <rdf:Description rdf:nodeID="autos421">
    <rdf:first>
      <owl:Class>
        <owl:complementOf rdf:resource="http://geographicknowledge.de/vocab/CoreConceptData.rdf#Raster" />
      </owl:Class>
    </rdf:first>
    <rdf:rest rdf:resource="http://www.w3.org/1999/02/22-rdf-syntax-ns#nil" />
  </rdf:Description>
  <rdf:Description rdf:nodeID="autos424">
    <rdf:first rdf:resource="http://geographicknowledge.de/vocab/CoreConceptData.rdf#Attribute" />
    <rdf:rest rdf:nodeID="autos425" />
  </rdf:Description>
  <rdf:Description rdf:nodeID="autos425">
    <rdf:first>
      <owl:Restriction>
        <owl:onProperty rdf:resource="http://geographicknowledge.de/vocab/AnalysisData.rdf#ofDataSet" />
        <owl:someValuesFrom rdf:resource="http://geographicknowledge.de/vocab/CoreConceptData.rdf#Vector" />
      </owl:Restriction>
    </rdf:first>
    <rdf:rest rdf:resource="http://www.w3.org/1999/02/22-rdf-syntax-ns#nil" />
  </rdf:Description>
  <rdf:Description rdf:nodeID="autos428">
    <rdf:first rdf:resource="http://geographicknowledge.de/vocab/CoreConceptData.rdf#RegionDS" />
    <rdf:rest rdf:nodeID="autos429" />
  </rdf:Description>
  <rdf:Description rdf:nodeID="autos429">
    <rdf:first rdf:resource="http://geographicknowledge.de/vocab/CoreConceptData.rdf#Vector" />
    <rdf:rest rdf:resource="http://www.w3.org/1999/02/22-rdf-syntax-ns#nil" />
  </rdf:Description>
  <rdf:Description rdf:nodeID="autos431">
    <rdf:first rdf:resource="http://geographicknowledge.de/vocab/CoreConceptData.rdf#RegionA" />
    <rdf:rest rdf:nodeID="autos432" />
  </rdf:Description>
  <rdf:Description rdf:nodeID="autos432">
    <rdf:first rdf:resource="http://geographicknowledge.de/vocab/CoreConceptData.rdf#VectorA" />
    <rdf:rest rdf:resource="http://www.w3.org/1999/02/22-rdf-syntax-ns#nil" />
  </rdf:Description>
  <rdf:Description rdf:nodeID="autos434">
    <rdf:first rdf:resource="http://geographicknowledge.de/vocab/CoreConceptData.rdf#Tessellation" />
    <rdf:rest rdf:nodeID="autos435" />
  </rdf:Description>
  <rdf:Description rdf:nodeID="autos435">
    <rdf:first rdf:resource="http://geographicknowledge.de/vocab/CoreConceptData.rdf#Vector" />
    <rdf:rest rdf:resource="http://www.w3.org/1999/02/22-rdf-syntax-ns#nil" />
  </rdf:Description>
  <rdf:Description rdf:nodeID="autos437">
    <rdf:first rdf:resource="http://geographicknowledge.de/vocab/CoreConceptData.rdf#TessellationA" />
    <rdf:rest rdf:nodeID="autos438" />
  </rdf:Description>
  <rdf:Description rdf:nodeID="autos438">
    <rdf:first rdf:resource="http://geographicknowledge.de/vocab/CoreConceptData.rdf#VectorA" />
    <rdf:rest rdf:resource="http://www.w3.org/1999/02/22-rdf-syntax-ns#nil" />
  </rdf:Description>
</rdf:RDF>